examples/crypto/cryptobox/Box.DH.fst
@@ -41,19 +41,19 @@ assume val hash: dh_element -> Tot aes_key
 (*
   Setting up a global log for AE.keys indexed by the ids of the public and private key involved.
 *)
-private type range = fun (k_id:ae_id) -> k:PlainDH.key{PlainDH.ae_key_get_index k = k_id}
-private let inv (f:MM.map' (ae_id) range) = True
+private type range = fun (k_id:id{AE_id? k_id}) -> k:PlainDH.key{PlainDH.ae_key_get_index k = k_id}
+private let inv (f:MM.map' (i:id{AE_id? i}) range) = True
 
 assume val ae_key_log_region: (r:HH.rid{ extends r root /\ is_eternal_region r /\ is_below r root})
 //private let ae_key_log_region = new_region root
-assume val ae_key_log: MM.t ae_key_log_region ae_id range inv
+assume val ae_key_log: MM.t ae_key_log_region (i:id{AE_id? i}) range inv
 //private let ae_key_log = MM.alloc #ae_key_log_region #ae_id #range #inv
 
 noeq abstract type dh_pkey = 
-  | DH_pkey:  #pk_id:id -> rawpk:dh_share -> dh_pkey
+  | DH_pkey:  #pk_id:id{DH_id? pk_id} -> rawpk:dh_share -> dh_pkey
 
 noeq abstract type dh_skey =
-  | DH_skey: #sk_id:id -> rawsk:dh_exponent -> pk:dh_pkey{pk.pk_id=sk_id} -> dh_skey 
+  | DH_skey: #sk_id:id{DH_id? sk_id} -> rawsk:dh_exponent -> pk:dh_pkey{pk.pk_id=sk_id} -> dh_skey 
 
 val sk_get_index: sk:dh_skey -> Tot (i:id{i = sk.sk_id})
 let sk_get_index k = k.sk_id
@@ -67,23 +67,28 @@ let pk_get_rawpk pk =
 
 assume val dh_exponentiate: dh_element -> dh_exponent -> Tot dh_element
 
-val keygen: #i:id -> ST (dh_pair:(k:dh_pkey{k.pk_id=i}) * (k:dh_skey{k.sk_id=i}))
-  (requires (fun h -> fresh i h))
+val keygen: #i:id{DH_id? i} -> ST (dh_pair:(k:dh_pkey{k.pk_id=i}) * (k:dh_skey{k.sk_id=i}))
+  (requires (fun h -> 
+    fresh i h
+    /\ fixed i
+  ))
   (ensures (fun h0 k h1 -> 
     unfresh i
+    /\ fixed i
   ))
 let keygen #i =
   let dh_share,dh_exponent = dh_gen_key() in
   let dh_pk = DH_pkey #i dh_share in
   let dh_sk = DH_skey #i dh_exponent dh_pk in
   make_unfresh i;
+  //make_honest i;
   dh_pk,dh_sk
 
-val coerce_pkey: #i:id{dishonest i} -> dh_share -> St (pk:dh_pkey{pk.pk_id=i})
+val coerce_pkey: #i:id{DH_id? i /\ dishonest i} -> dh_share -> St (pk:dh_pkey{pk.pk_id=i})
 let coerce_pkey #i dh_sh =
   DH_pkey #i dh_sh
 
-val coerce_keypair: #i:id{dishonest i} -> dh_exponent -> St (dh_pair:(k:dh_pkey{k.pk_id=i}) * (k:dh_skey{k.sk_id=i}))
+val coerce_keypair: #i:id{DH_id? i /\ dishonest i} -> dh_exponent -> St (dh_pair:(k:dh_pkey{k.pk_id=i}) * (k:dh_skey{k.sk_id=i}))
 let coerce_keypair #i dh_ex =
   let dh_sh = dh_exponentiate dh_base dh_ex in
   let pk = DH_pkey #i dh_sh in
@@ -112,22 +117,22 @@ let prf_odhT dh_sk dh_pk =
 val prf_odh: sk:dh_skey -> pk:dh_pkey -> ST (PlainDH.key)
   ( requires (fun h0 ->
     let i = generate_ae_id pk.pk_id sk.sk_id in
-    ae_fixed i
-    /\ (ae_honest i \/ ae_dishonest i)
+    fixed i
+    /\ (honest i \/ dishonest i)
   ))
   ( ensures (fun h0 k h1 ->
     let i = generate_ae_id pk.pk_id sk.sk_id in
     let s:Set.set (r:HH.rid) = Set.union (Set.singleton ae_key_log_region) (Set.singleton (leak_regionGT k)) in
     (PlainDH.ae_key_get_index k = i)
-    /\ (ae_honest i \/ ae_dishonest i)
+    /\ (honest i \/ dishonest i)
     /\ (
-        ( (ae_honest i /\ prf_odh)
+        ( (honest i /\ prf_odh)
     	    ==> (modifies s h0 h1
     	       /\ MR.witnessed (MM.contains ae_key_log i k) 
     	      )
         )
         \/ 
-    	( (ae_dishonest i \/ ~prf_odh)
+    	( (dishonest i \/ ~prf_odh)
     	    ==> (modifies_one (PlainDH.leak_regionGT k) h0 h1
     	       /\ leak_key k = prf_odhT sk pk
     	      )
@@ -135,13 +140,16 @@ val prf_odh: sk:dh_skey -> pk:dh_pkey -> ST (PlainDH.key)
       )
   ))
 
+// Proposal: Move the ae_key_log to Box.AE and have AE.keygen guarantee that they output unique keys per ID.
+// Prf-odh can then branch on the prf_odh flag and the honesty of the ae_id to decide if it wants to use keygen
+// or coerce_key. This could break consistency with the formal model. Reduction needed?
 // Prove memory-safety for prf_odh
 let prf_odh dh_sk dh_pk =
   let pk_id = dh_pk.pk_id in
   let sk_id = dh_sk.sk_id in
   let i = generate_ae_id pk_id sk_id in
-  let ae_honest_i = ae_honestST i in
-  if ae_honest_i && prf_odh then
+  let honest_i = honestST i in
+  if honest_i && prf_odh then
     (MR.m_recall ae_key_log;
     let entry = MM.lookup ae_key_log i in
     match entry with
@@ -152,7 +160,7 @@ let prf_odh dh_sk dh_pk =
       MM.extend ae_key_log i k';
       k')
   else(
-    assert(ae_dishonest i \/ ~prf_odh);
+    assert(dishonest i \/ ~prf_odh);
     let raw_k = dh_exponentiate dh_pk.rawpk dh_sk.rawsk in
     let hashed_raw_k = hash raw_k in
     assume(disjoint ae_key_region ae_key_log_region);
