examples/crypto/cryptobox/Box.Indexing.fst
@@ -8,8 +8,25 @@ open FStar.HyperStack
 module MR = FStar.Monotonic.RRef
 module MM = MonotoneMap
 
-type id = int
+type dh_id = int
+abstract type ae_id = (i:(dh_id*dh_id){fst i <= snd i})
+
+type id =
+  | DH_id of dh_id
+  | AE_id of ae_id
+
+val generate_ae_id: i1:id{DH_id? i1} -> i2:id{DH_id? i2} -> Tot (i3:id{AE_id? i3})
+let generate_ae_id i1 i2 =
+  match i1,i2 with
+  | DH_id i1',DH_id i2' ->
+  if i1' <= i2' then
+    AE_id (i1',i2')
+  else
+    AE_id (i2',i1')
+
+
 assume Index_hasEq: hasEq id
+assume AE_Index_hasEq: hasEq ae_id
 
 type id_freshness_table_key = id
 type id_freshness_table_value = unit
@@ -20,24 +37,24 @@ assume val id_freshness_table_region: (r:MR.rid{extends r root /\ is_eternal_reg
 
 assume val id_freshness_table: MM.t id_freshness_table_region id_freshness_table_key id_freshness_table_range id_freshness_table_inv
 
-type id_honesty_table_key = id
+
+type id_honesty_table_key = dh_id
 type id_honesty_table_value = bool
 type id_honesty_table_range = fun id_honesty_table_key -> id_honesty_table_value
 let id_honesty_table_inv (m:MM.map' id_honesty_table_key id_honesty_table_range) = 
-  forall i. Some? (MM.sel m i) ==> MR.witnessed (MM.defined id_freshness_table i)
+  forall i. Some? (MM.sel m i) ==> MR.witnessed (MM.defined id_freshness_table (DH_id i))
        
-assume val id_honesty_table_region: (r:MR.rid{ extends r root /\ is_eternal_region r /\ is_below r root})
+assume val id_honesty_table_region: (r:MR.rid{ extends r root /\ is_eternal_region r /\ is_below r root /\ disjoint r id_freshness_table_region})
 //let id_table_region = new_region root in
 
 assume val id_honesty_table: MM.t id_honesty_table_region id_honesty_table_key id_honesty_table_range id_honesty_table_inv
 //let id_table = MM.alloc #id_table_region #id #range #inv in
 
-val fresh: (i:id) -> h:mem -> Tot Type0
 let fresh (i:id) h =
-  MM.contains id_freshness_table i () h
+  ~(MM.defined id_freshness_table i h)
 
 type unfresh (i:id) =
-  MR.witnessed (MM.contains id_freshness_table i ())
+  MR.witnessed (MM.defined id_freshness_table i)
 
 val make_unfresh: (i:id) -> ST (unit)
   (requires (fun h0 -> True))
@@ -50,72 +67,85 @@ let make_unfresh i =
   match MM.lookup id_freshness_table i with
   | Some i' -> ()
   | None ->
-    MM.extend id_freshness_table i ();
-    ()
+    MM.extend id_freshness_table i ()
 
-type honest (i:id) =
-  MR.witnessed (MM.contains id_honesty_table i true)
+private let measure_id (i:id) =
+  match i with
+  | DH_id i' -> 0
+  | _ -> 1
 
-type dishonest (i:id) =
-  MR.witnessed (MM.contains id_honesty_table i false)
+val honest: (i:id) -> Tot (Type0) (decreases (measure_id i))
+let rec honest (i:id) =
+  match i with
+  | DH_id i' -> MR.witnessed (MM.contains id_honesty_table i' true)
+  | AE_id (i1,i2) -> honest (DH_id i1) /\ honest (DH_id i2)
 
-type fixed (i:id) =
-  MR.witnessed (MM.defined id_honesty_table i)
+val dishonest: (i:id) -> Tot Type0 (decreases (measure_id i))
+let rec dishonest (i:id) =
+  match i with
+  | DH_id i' -> MR.witnessed (MM.contains id_honesty_table i' false)
+  | AE_id (i1,i2) -> dishonest (DH_id i1) \/ dishonest (DH_id i2)
 
+val fixed: (i:id) -> Tot Type0 (decreases (measure_id i))
+let rec fixed (i:id) =
+  match i with
+  | DH_id i' -> MR.witnessed (MM.defined id_honesty_table i')
+  | AE_id (i1,i2) -> fixed (DH_id i1) /\ fixed (DH_id i2)
 
-val make_dishonest: (i:id) -> ST (unit)
-  (requires (fun h0 -> 
-    MR.witnessed (MM.defined id_freshness_table i)
-    /\ MM.fresh id_honesty_table i h0
-  ))
-  (ensures (fun h0 _ h1 -> dishonest i))
-let make_dishonest i =
-  MM.extend id_honesty_table i false;
-  ()
+// Implement these two for the adversary
+//val make_dishonest: (i:id) -> ST (unit) (decreases (measure_id i))
+//  (requires (fun h0 -> 
+//    unfresh i
+//  ))
+//  (ensures (fun h0 _ h1 -> dishonest i))
+//let rec make_dishonest i =
+//  MR.m_recall id_honesty_table;
+//  match i with
+//  | DH_id i' -> (
+//    match MM.lookup id_honesty_table i' with
+//    | Some v -> ()
+//    | None -> MM.extend id_honesty_table i' false)
+//  | AE_id (i1,i2) -> 
+//    make_dishonest (DH_id i1);
+//    make_dishonest (DH_id i2)
+    
 
-val make_honest: (i:id) -> ST (unit)
-  (requires (fun h0 ->
-    MR.witnessed (MM.defined id_freshness_table i)
-    /\ MM.fresh id_honesty_table i h0
-  ))
-  (ensures (fun h0 _ h1 -> honest i))
-let make_honest i =
-  MM.extend id_honesty_table i true;
-  ()
-  
+//val make_honest: (i:id) -> ST (unit)
+//  (requires (fun h0 ->
+//    unfresh i
+//    /\ MM.fresh id_honesty_table i h0
+//  ))
+//  (ensures (fun h0 _ h1 -> honest i))
+//let make_honest i =
+//  MR.m_recall id_honesty_table;
+//  MM.extend id_honesty_table i true;
+//  ()
 
-val honestST: i:id{fixed i} -> ST(b:bool{(b ==> honest i) /\ (not b ==> dishonest i)})
+val honestST: i:id{fixed i} -> ST(b:bool{(b ==> honest i) /\ (not b ==> dishonest i)}) (decreases (measure_id i))
   (requires (fun h0 -> True))
   (ensures (fun h0 b h1 ->
     modifies_none h0 h1 
     /\ MR.m_contains id_honesty_table h1
   ))
-let honestST i =
+let rec honestST i =
   MR.m_recall id_honesty_table;
-  MR.testify(MM.defined id_honesty_table i);
-  match MM.lookup id_honesty_table i with
-  |Some v -> 
-    v
+  match i with
+  | DH_id i' -> (
+    MR.testify (MM.defined id_honesty_table i');
+    match MM.lookup id_honesty_table i' with
+    |Some v -> 
+      v)
+  | AE_id (i1,i2) -> 
+    let b1 = honestST (DH_id i1) in
+    let b2 = honestST (DH_id i2) in
+    b1 && b2
+  
 
-abstract type ae_id = 
-  | AE_id: i:(id*id){fst i <= snd i} -> ae_id
-
-val generate_ae_id: i1:id -> i2:id -> Tot (i3:ae_id{fst i3.i <= snd i3.i})
-let generate_ae_id i1 i2 =
-  if i1 <= i2 then
-    AE_id (i1,i2)
-  else
-    AE_id (i2,i1)
-
-val unique_id_generation: i1:id -> i2:id -> Lemma
-  (requires (True))
-  (ensures (forall id1 id2. generate_ae_id id1 id2 = generate_ae_id id2 id1))
-  [SMTPat (generate_ae_id i1 i2)]
-let unique_id_generation i1 i2 = ()
-
-val honest_dishonest_lemma: i:id -> ST(unit)
-  (requires (fun h -> fixed i))
-  (ensures (fun h0 _ h1 -> modifies_none h0 h1 /\
+val honest_dishonest_lemma: dh_i:dh_id -> ST(unit)
+  (requires (fun h -> fixed (DH_id dh_i)))
+  (ensures (fun h0 _ h1 ->
+    let i = DH_id dh_i in
+    modifies_none h0 h1 /\
     ( dishonest i \/ honest i ) /\
     ( ~(honest i) ==> dishonest i ) /\
     ( ~(dishonest i) ==> honest i ) /\
@@ -128,8 +158,8 @@ let honest_dishonest_lemma i =
   match MM.lookup id_honesty_table i with
   |Some v -> ()
 
-val honest_dishonest_contradiction_lemma: i:id -> ST(unit)
-  (requires (fun h -> honest i /\ dishonest i))
+val honest_dishonest_contradiction_lemma: i:dh_id -> ST(unit)
+  (requires (fun h -> honest (DH_id i) /\ dishonest (DH_id i)))
   (ensures (fun h0 _ h1 -> False
   ))
 let honest_dishonest_contradiction_lemma i = 
@@ -137,47 +167,74 @@ let honest_dishonest_contradiction_lemma i =
   MR.testify(MM.contains id_honesty_table i false);
   ()
 
-type ae_fresh i h =
-  fresh (fst i.i) h /\ fresh (snd i.i) h
+
+////////////////////////////////////////////////////////////////////////////////////////////////
+//  Data type and functions of ae_id, which is composed of two regular ids.
+///////////////////////////////////////////////////////////////////////////////////////////////
+
+//let ae_fresh i h =
+//  ~(MM.defined id_freshness_table i h)
+
+
+//type ae_unfresh (i:ae_id) =
+//  MR.witnessed (MM.defined id_freshness_table i)
+
+//val ae_make_unfresh: (i:ae_id) -> ST (unit)
+//  (requires (fun h0 -> True))
+//  (ensures (fun h0 _ h1 ->
+//    modifies (Set.singleton id_freshness_table_region) h0 h1
+//    /\ ae_unfresh i
+//  ))
+//let ae_make_unfresh i =
+//  MR.m_recall id_freshness_table;
+//  match MM.lookup id_freshness_table i with
+//  | Some v -> ()
+//  | None -> 
+//    MM.extend id_freshness_table i ()
   
-
-type ae_unfresh (i:ae_id) =
-  unfresh (fst i.i) /\ unfresh (snd i.i)
-
-val ae_make_unfresh: (i:ae_id) -> ST (unit)
-  (requires (fun h0 -> True))
-  (ensures (fun h0 _ h1 ->
-    modifies (Set.singleton id_freshness_table_region) h0 h1
-    /\ ae_unfresh i
-  ))
-let ae_make_unfresh i =
-  make_unfresh (fst i.i);
-  make_unfresh (snd i.i);
-  ()
-  
-type ae_honest k_i =
-  honest (fst k_i.i) /\ honest (snd k_i.i)
-
-type ae_dishonest (k_i:ae_id) =
-  dishonest (fst k_i.i) \/ dishonest (snd k_i.i)
-
-type ae_fixed (k_i:ae_id) = 
-  fixed (fst k_i.i) /\ fixed(snd k_i.i)
-  
-
-
-val ae_honestST: k_i:ae_id{ae_fixed k_i} -> ST(b:bool{(b ==> (ae_honest k_i)) /\ (not b ==> (ae_dishonest k_i))})
-  (requires (fun h0 -> True))
-  (ensures (fun h0 b h1 ->
-    modifies_none h0 h1
-    /\ MR.m_contains id_honesty_table h1
-    /\ (ae_honest k_i \/ ae_dishonest k_i)
-    /\ ae_fixed k_i
-  ))
-let ae_honestST k_i =
-  let h1 = honestST (fst k_i.i) in 
-  let h2 = honestST (snd k_i.i) in
-  (h1 && h2)
+//type ae_honest k_i =
+//  honest (fst k_i) /\ honest (snd k_i)
+//
+//type ae_dishonest (k_i:ae_id) =
+//  dishonest (fst k_i) \/ dishonest (snd k_i)
+//
+//type ae_fixed (k_i:ae_id) = 
+//  fixed (fst k_i) /\ fixed(snd k_i)
+//  
+//val ae_make_honest: i:ae_id -> ST unit
+//  (requires (fun h0 -> honest i))
+//  (ensures (fun h0 _ h1 ->
+//    ae_honest i
+//  ))
+//
+//val ae_honestST: k_i:ae_id{ae_fixed k_i} -> ST(b:bool{(b ==> (ae_honest k_i)) /\ (not b ==> (ae_dishonest k_i))})
+//  (requires (fun h0 -> True))
+//  (ensures (fun h0 b h1 ->
+//    modifies_none h0 h1
+//    /\ MR.m_contains id_honesty_table h1
+//    /\ (ae_honest k_i \/ ae_dishonest k_i)
+//    /\ ae_fixed k_i
+//  ))
+//let ae_honestST k_i =
+//  let h1 = honestST (fst k_i) in 
+//  let h2 = honestST (snd k_i) in
+//  (h1 && h2)
 
 
+val unique_id_generation: i1:id{AE_id? i1} -> i2:id{AE_id? i2} -> Lemma
+  (requires (True))
+  (ensures (forall id1 id2. generate_ae_id id1 id2 = generate_ae_id id2 id1))
+  [SMTPat (generate_ae_id i1 i2)]
+let unique_id_generation i1 i2 = ()
 
+//val ae_id_property_lemma: (i1:id) -> (i2:id) -> Lemma
+//  (requires True)
+//  (ensures (
+//    let i3 = generate_ae_id i1 i2 in
+//    (fixed i1 /\ fixed i2 ==> ae_fixed i3)
+//    /\ (honest i1 /\ honest i2 ==> ae_honest i3)
+//    /\ (dishonest i1 \/ dishonest i2 ==> ae_dishonest i3)
+//  ))
+//  [SMTPat (generate_ae_id i1 i2)]
+//let ae_id_property_lemma i1 i2 = ()
+//
