examples/crypto/cryptobox/Box.PlainPKAE.fst
@@ -11,25 +11,25 @@ open FStar.Monotonic.RRef
 open Platform.Bytes
 
 
-abstract type protected_pkae_plain = 
-  | Prot_pkae_p: #i:ae_id -> b:bytes -> protected_pkae_plain
+noeq abstract type protected_pkae_plain = 
+  | Prot_pkae_p: #i:id{AE_id? i} -> b:bytes -> protected_pkae_plain
 //assume Plain_hasEq: hasEq protected_pkae_plain
 type pkae_plain = bytes
 
-val get_index: p:protected_pkae_plain -> Tot (i:ae_id{i=p.i})
+val get_index: p:protected_pkae_plain -> Tot (i:id{i=p.i})
 let get_index p =
   p.i
 
 (* two pure functions, never called when ideal *)
-val repr: p:protected_pkae_plain{not pkae \/ (ae_dishonest p.i) } -> Tot pkae_plain
+val repr: p:protected_pkae_plain{not pkae \/ (dishonest p.i) } -> Tot pkae_plain
 let repr p = p.b
 
 // Change this if we want to use signcryption with pkae_int-ctxt
-val coerce: #i:ae_id -> p:pkae_plain{not pkae \/ (ae_dishonest i)} -> Tot (prot:protected_pkae_plain{i=prot.i})
+val coerce: #i:id{AE_id? i} -> p:pkae_plain{not pkae \/ (dishonest i)} -> Tot (prot:protected_pkae_plain{i=prot.i})
 let coerce #i p = 
   Prot_pkae_p #i p  
 
-val length: #i:ae_id -> protected_pkae_plain -> Tot nat
-let length #i p = length p.b
+val length:  protected_pkae_plain -> Tot nat
+let length p = length p.b
 
 // Create coece_keyshare function
